src/program_proof/new_proof_prelude.v
@@ -1,0 +1,20 @@
+From iris.algebra Require Export auth gmap frac agree excl vector.
+
+From Perennial.algebra Require Export big_op.
+
+From Perennial.Helpers Require Export Tactics List ListLen BigOp Transitions iris ipm.
+
+From Perennial.base_logic Require Export ghost_var.
+From Perennial.program_logic Require Export ncinv.
+From Perennial.goose_lang Require Export proofmode wpc_proofmode array.
+From Perennial.goose_lang Require Export into_val.
+From Perennial.goose_lang.lib Require Export
+     persistent_readonly slice slice.typed_slice struct control map.typed_map time proph rand string.
+From Perennial.goose_lang.new Require Export loop exception exception_wps.
+
+Export uPred.
+
+Global Set Default Proof Using "Type".
+Global Set Printing Projections.
+
+Global Opaque load_ty store_ty.
